Add the unit type

src/Log.v
@@ -1,10 +1,8 @@
 Set Warnings "-cannot-remove-as-expected".
 
 Require Import
-  Coq.Unicode.Utf8
-  Coq.Program.Program
-  Coq.Classes.CRelationClasses
-  Coq.Classes.Morphisms
+  Lib
+  Ltac
   Ty
   Exp
   Sub.
@@ -25,10 +23,10 @@ Variable P : ∀ {τ}, Exp Γ τ → Prop.
 (** [ExpP] is a logical predicate that permits type-directed induction on
     expressions. *)
 Equations ExpP `(e : Exp Γ τ) : Prop :=
-  ExpP (τ:=_ ⟶ _) f := P f ∧ (∀ x, ExpP x → ExpP (APP f x)).
+  ExpP (τ:=_ ⟶ _) f := P f ∧ (∀ x, ExpP x → ExpP (APP f x));
   (* ExpP (τ:=_ × _)    p := P p ∧ ExpP (Fst p) ∧ ExpP (Snd p); *)
   (* ExpP (τ:=TyList _) l := P l ∧ (∀ d, ExpP d → ExpP (Car d l)); *)
-  (* ExpP e := P e. *)
+  ExpP e := P e.
 
 Inductive SubP : ∀ {Γ'}, Sub Γ Γ' → Prop :=
   | NoSubP : SubP (NoSub (Γ:=Γ))
@@ -39,5 +37,17 @@ Derive Signature for SubP.
 
 Lemma ExpP_P {τ} {e : Γ ⊢ τ} : ExpP e → P e.
 Proof. intros; induction τ; simpl in *; simp ExpP in H; now reduce. Qed.
+
+Variable R : ∀ {τ}, Exp Γ τ → Exp Γ τ → Prop.
+
+(** [ExpR] is a logical predicate that permits type-directed induction on
+    expressions. *)
+Equations ExpR {τ} (e1 e2 : Exp Γ τ) : Prop :=
+  ExpR (τ:=_ ⟶ _) f1 f2 :=
+    R f1 f2 ∧ (∀ x1 x2, ExpR x1 x2 → ExpR (APP f1 x1) (APP f1 x1));
+  ExpR e1 e2 := R e1 e2.
+
+Lemma ExpR_P {τ} {e1 e2 : Γ ⊢ τ} : ExpR e1 e2 → R e1 e2.
+Proof. intros; induction τ; simpl in *; simp ExpR in H; now reduce. Qed.
 
 End Log.
